books/str/iless.lisp
@@ -20,57 +20,8 @@
 
 (in-package "STR")
 (include-book "ieqv")
-(include-book "char-case")
 (local (include-book "unicode/nthcdr" :dir :system))
 (local (include-book "arithmetic"))
-
-
-(local
- (encapsulate
-   ()
-   (local (defund exhaustive-test (n)
-            (and (let ((x (code-char n)))
-                   (implies (and (<= 65 (char-code x))
-                                 (<= (char-code x) 90))
-                            (and (standard-char-p x)
-                                 (standard-char-p (code-char (+ (char-code x) 32))))))
-                 (or (zp n)
-                     (exhaustive-test (- n 1))))))
-
-   (local (defthm lemma
-            (implies (and (natp n)
-                          (natp m)
-                          (exhaustive-test n)
-                          (= x (code-char m))
-                          (<= m n)
-                          (<= n 255))
-                     (implies (and (<= 65 (char-code x))
-                                   (<= (char-code x) 90))
-                              (and (standard-char-p x)
-                                   (standard-char-p (code-char (+ (char-code x) 32))))))
-            :hints(("goal"
-                    :induct (exhaustive-test n)
-                    :in-theory (enable exhaustive-test)))))
-
-   (defthm standard-char-p-when-upper-case
-     (implies (and (<= 65 (char-code x))
-                   (<= (char-code x) 90))
-              (standard-char-p x))
-     :hints(("Goal"
-             :in-theory (disable lemma)
-             :use ((:instance lemma
-                              (n 255)
-                              (m (char-code x)))))))
-
-   (defthm standard-char-p-of-char-downcase
-     (implies (and (<= 65 (char-code x))
-                   (<= (char-code x) 90))
-              (standard-char-p (code-char (+ 32 (char-code x)))))
-     :hints(("goal"
-             :in-theory (disable lemma)
-             :use ((:instance lemma
-                              (n 255)
-                              (m (char-code x)))))))))
 
 
 (defsection ichar<
@@ -89,33 +40,22 @@ hat, underscore, and backtick) are considered \"smaller\" than letters, even
 though in regular ASCII ordering they are \"larger\" than the upper-case
 letters.</p>"
 
-  (defund ichar< (x y)
+  (definlined ichar< (x y)
     (declare (type character x)
-             (type character y))
+             (type character y)
+             (xargs :guard-hints(("Goal" :in-theory (enable downcase-char)))))
     (mbe :logic
-         (let* ((xc (if (characterp x)
-                        (char-code x)
-                      0))
-                (yc (if (characterp y)
-                        (char-code y)
-                      0))
-                (xc-fix (if (and (<= (char-code #\A) xc) (<= xc (char-code #\Z)))
-                            (+ xc 32)
-                          xc))
-                (yc-fix (if (and (<= (char-code #\A) yc) (<= yc (char-code #\Z)))
-                            (+ yc 32)
-                          yc)))
-           (< xc-fix yc-fix))
-
+         (< (char-code (downcase-char x))
+            (char-code (downcase-char y)))
          :exec
-         (let* ((xc     (the (unsigned-byte 8) (char-code (the character x))))
-                (yc     (the (unsigned-byte 8) (char-code (the character y))))
-                (xc-fix (if (and (<= (the (unsigned-byte 8) 65) (the (unsigned-byte 8) xc))
-                                 (<= (the (unsigned-byte 8) xc) (the (unsigned-byte 8) 90)))
+         (let* ((xc (the (unsigned-byte 8) (char-code (the character x))))
+                (yc (the (unsigned-byte 8) (char-code (the character y))))
+                (xc-fix (if (and (<= (big-a) (the (unsigned-byte 8) xc))
+                                 (<= (the (unsigned-byte 8) xc) (big-z)))
                             (the (unsigned-byte 8) (+ (the (unsigned-byte 8) xc) 32))
                           (the (unsigned-byte 8) xc)))
-                (yc-fix (if (and (<= (the (unsigned-byte 8) 65) (the (unsigned-byte 8) yc))
-                                 (<= (the (unsigned-byte 8) yc) (the (unsigned-byte 8) 90)))
+                (yc-fix (if (and (<= (big-a) (the (unsigned-byte 8) yc))
+                                 (<= (the (unsigned-byte 8) yc) (big-z)))
                             (the (unsigned-byte 8) (+ (the (unsigned-byte 8) yc) 32))
                           (the (unsigned-byte 8) yc))))
            (< (the (unsigned-byte 8) xc-fix)
@@ -140,44 +80,34 @@ letters.</p>"
                   (ichar< x y))
              (ichar< x z)))
 
-  (encapsulate
-    ()
-    (local (defthm lemma
-             (implies (and (<= 65 (char-code x))
-                           (<= (char-code x) 90)
-                           (equal (char-code y) (+ 32 (char-code x))))
-                      (standard-char-p y))
-             :hints(("Goal"
-                     :in-theory (disable standard-char-p-of-char-downcase)
-                     :use ((:instance standard-char-p-of-char-downcase))))))
-
-    (defthm ichar<-trichotomy-weak
-      (implies (and (not (ichar< x y))
-                    (not (ichar< y x)))
-               (equal (ichareqv x y)
-                      t))
-      :hints(("Goal" :in-theory (enable ichar<
-                                        ichareqv
-                                        downcase-char)))))
+  (defthm ichar<-trichotomy-weak
+    (implies (and (not (ichar< x y))
+                  (not (ichar< y x)))
+             (equal (ichareqv x y)
+                    t))
+    :hints(("Goal" :in-theory (enable ichar<
+                                      ichareqv
+                                      downcase-char
+                                      char-fix))))
 
   (defcong ichareqv equal (ichar< x y) 1
     :hints(("Goal" :in-theory (enable ichar<
                                       ichareqv
                                       downcase-char
-                                      standard-char-p-of-char-downcase))))
+                                      char-fix))))
 
   (defcong ichareqv equal (ichar< x y) 2
     :hints(("Goal" :in-theory (enable ichar<
                                       ichareqv
                                       downcase-char
-                                      standard-char-p-of-char-downcase))))
+                                      char-fix))))
 
   (defthm ichar<-trichotomy-strong
     (equal (ichar< x y)
            (and (not (ichareqv x y))
                 (not (ichar< y x))))
     :hints(("Goal"
-            :in-theory (e/d (ichareqv downcase-char)
+            :in-theory (e/d (ichareqv downcase-char char-fix)
                             (ichar<-trichotomy-weak))
             :use ((:instance ichar<-trichotomy-weak))))
     :rule-classes ((:rewrite :loop-stopper ((x y))))))
@@ -215,12 +145,12 @@ smaller than longer strings.</p>"
                (t
                 (let* ((xc     (the (unsigned-byte 8) (char-code (the character (car x)))))
                        (yc     (the (unsigned-byte 8) (char-code (the character (car y)))))
-                       (xc-fix (if (and (<= (the (unsigned-byte 8) 65) (the (unsigned-byte 8) xc))
-                                        (<= (the (unsigned-byte 8) xc) (the (unsigned-byte 8) 90)))
+                       (xc-fix (if (and (<= (big-a) (the (unsigned-byte 8) xc))
+                                        (<= (the (unsigned-byte 8) xc) (big-z)))
                                    (the (unsigned-byte 8) (+ (the (unsigned-byte 8) xc) 32))
                                  (the (unsigned-byte 8) xc)))
-                       (yc-fix (if (and (<= (the (unsigned-byte 8) 65) (the (unsigned-byte 8) yc))
-                                        (<= (the (unsigned-byte 8) yc) (the (unsigned-byte 8) 90)))
+                       (yc-fix (if (and (<= (big-a) (the (unsigned-byte 8) yc))
+                                        (<= (the (unsigned-byte 8) yc) (big-z)))
                                    (the (unsigned-byte 8) (+ (the (unsigned-byte 8) yc) 32))
                                  (the (unsigned-byte 8) yc))))
                   (cond ((< (the (unsigned-byte 8) xc-fix) (the (unsigned-byte 8) yc-fix))
@@ -233,7 +163,7 @@ smaller than longer strings.</p>"
   (local (in-theory (enable icharlist<)))
 
   (verify-guards icharlist<
-    :hints(("Goal" :in-theory (e/d (ichar<)
+    :hints(("Goal" :in-theory (e/d (ichar< downcase-char)
                                    (ichar<-trichotomy-strong)))))
 
   (defthm icharlist<-irreflexive
@@ -325,12 +255,12 @@ into lists.</p>
                        (yc     (the (unsigned-byte 8)
                                  (char-code (the character
                                               (char (the string y) (the integer n))))))
-                       (xc-fix (if (and (<= (the (unsigned-byte 8) 65) (the (unsigned-byte 8) xc))
-                                        (<= (the (unsigned-byte 8) xc) (the (unsigned-byte 8) 90)))
+                       (xc-fix (if (and (<= (big-a) (the (unsigned-byte 8) xc))
+                                        (<= (the (unsigned-byte 8) xc) (big-z)))
                                    (the (unsigned-byte 8) (+ (the (unsigned-byte 8) xc) 32))
                                  (the (unsigned-byte 8) xc)))
-                       (yc-fix (if (and (<= (the (unsigned-byte 8) 65) (the (unsigned-byte 8) yc))
-                                        (<= (the (unsigned-byte 8) yc) (the (unsigned-byte 8) 90)))
+                       (yc-fix (if (and (<= (big-a) (the (unsigned-byte 8) yc))
+                                        (<= (the (unsigned-byte 8) yc) (big-z)))
                                    (the (unsigned-byte 8) (+ (the (unsigned-byte 8) yc) 32))
                                  (the (unsigned-byte 8) yc))))
                   (cond ((< (the (unsigned-byte 8) xc-fix) (the (unsigned-byte 8) yc-fix))
@@ -344,7 +274,7 @@ into lists.</p>
                                     (the integer xl)
                                     (the integer yl)))))))))
 
-  (defun istr< (x y)
+  (definline istr< (x y)
     (declare (type string x)
              (type string y)
              (xargs :verify-guards nil))
@@ -358,12 +288,17 @@ into lists.</p>
                     (the integer (length (the string x)))
                     (the integer (length (the string y))))))
 
-  (local (in-theory (enable istr<-aux
-                            istr<)))
+  (local (defthm crock
+           (equal (< a a)
+                  nil)))
+
+  (local (defthm crock2
+           (implies (< a b)
+                    (equal (< b a)
+                           nil))))
 
   (verify-guards istr<-aux
-    :hints(("Goal" :in-theory (e/d (ichar<)
-                                   (ichar<-trichotomy-strong)))))
+    :hints(("Goal" :in-theory (e/d (ichar< downcase-char)))))
 
   (defthm istr<-aux-correct
     (implies (and (stringp x)
@@ -378,5 +313,5 @@ into lists.</p>
                                 (nthcdr n (coerce y 'list)))))
     :hints(("Goal" :in-theory (enable istr<-aux icharlist<))))
 
-  (verify-guards istr<))
+  (verify-guards istr<$inline))
 
